src/verified_adapter.ml
@@ -141,15 +141,16 @@ let unorderedFlatMap m =
 
 let convert_db md =
   let rbt_single x = RBT_set (rbt_insert x rbt_empty) in
+  let convert_cst' x = Some (convert_cst x) in
   let add_builtin xs (name, tup) =
     let arity = nat_of_int (List.length tup) in
-    ((name, arity), rbt_single (List.map convert_cst tup)) :: xs
+    ((name, arity), rbt_single (List.map convert_cst' tup)) :: xs
   in
   let convert_table t =
     let (name, attrs) = (Table.get_schema t) in
     let arity = nat_of_int (List.length attrs) in
     ((name, arity), RBT_set (Relation.fold
-      (fun v -> rbt_insert (List.map convert_cst v))
+      (fun v -> rbt_insert (List.map convert_cst' v))
       (Table.get_relation t) rbt_empty))
   in
   let db_events = List.map convert_table (Db.get_tables md.db) in
